more

Weidenbach_Book/Watched_Literals_List.thy
@@ -28,6 +28,9 @@ fun clauses_to_update_l :: \<open>'v twl_st_l \<Rightarrow> 'v clauses_to_update
 fun get_trail_l :: \<open>'v twl_st_l \<Rightarrow> ('v, nat) ann_lit list\<close> where
   \<open>get_trail_l (M, _, _, _, _, _, _, _) = M\<close>
 
+fun get_learned_l :: \<open>'v twl_st_l \<Rightarrow> nat\<close> where
+  \<open>get_learned_l (_, _, U, _, _, _, _, _) = U\<close>
+
 fun set_clauses_to_update_l :: \<open>'v clauses_to_update_l \<Rightarrow> 'v twl_st_l \<Rightarrow> 'v twl_st_l\<close> where
   \<open>set_clauses_to_update_l WS (M, N, U, D, NE, UE, _, Q) = (M, N, U, D, NE, UE, WS, Q)\<close>
 
@@ -73,9 +76,6 @@ lemma convert_lits_l_append[simp]:
   \<open>convert_lits_l N (M @ M') = convert_lits_l N M @ convert_lits_l N M'\<close>
   by (auto simp: convert_lits_l_def)
 
-
-fun get_learned_l :: \<open>'v twl_st_l \<Rightarrow> nat\<close> where
-  \<open>get_learned_l (_, _, U, _, _, _, _, _) = U\<close>
 
 abbreviation resolve_cls_l where
   \<open>resolve_cls_l L D' E \<equiv> union_mset_list (remove1 (-L) D') (remove1 L E)\<close>
@@ -1229,7 +1229,7 @@ qed
 
 lemma get_conflict_l_get_conflict_state_spec:
   assumes \<open>S' = twl_st_of None S\<close> and \<open>twl_list_invs S\<close> and \<open>clauses_to_update_l S = {#}\<close>
-  shows \<open>((get_conflict_l S = Some {#}, S), (get_conflict S' = Some {#}, S'))
+  shows \<open>((False, S), (False, S'))
   \<in> {((brk, S), (brk', S')). brk = brk' \<and> S' = twl_st_of None S \<and> twl_list_invs S \<and>
     clauses_to_update_l S = {#}}\<close>
   using assms by auto
@@ -1277,7 +1277,7 @@ definition skip_and_resolve_loop_l :: \<open>'v twl_st_l \<Rightarrow> 'v twl_st
                 do {RETURN (True, S)}
           }
         )
-        (get_conflict_l S\<^sub>0 = Some {#}, S\<^sub>0);
+        (False, S\<^sub>0);
       RETURN S
     }
   \<close>
@@ -1366,7 +1366,8 @@ lemma skip_and_resolve_loop_l_spec:
     {(S::'v twl_st_l, S'). S' = twl_st_of None S \<and> twl_struct_invs (twl_st_of None S) \<and>
        twl_stgy_invs (twl_st_of None S) \<and>
        twl_list_invs S \<and> clauses_to_update_l S = {#} \<and> literals_to_update_l S = {#} \<and>
-       get_conflict (twl_st_of None S) \<noteq> None} \<rightarrow>
+       get_conflict (twl_st_of None S) \<noteq> None \<and>
+       0 < count_decided (get_trail_l S)} \<rightarrow>
   \<langle>{(T, T'). T' = twl_st_of None T \<and> twl_list_invs T \<and>
     (twl_struct_invs (twl_st_of None T) \<and> twl_stgy_invs (twl_st_of None T) \<and>
     no_step cdcl\<^sub>W_restart_mset.skip (state\<^sub>W_of (twl_st_of None T)) \<and>
@@ -1414,13 +1415,22 @@ proof -
     by (intro ext) (auto simp: get_maximum_level_cong)
   have [simp]: \<open>count_decided (get_trail_l S) = count_decided (get_trail (twl_st_of None S))\<close> for S
     by (cases S) auto
+  have [simp]: \<open>get_trail_l S \<noteq> [] \<Longrightarrow> tl_state (twl_st_of None S) = twl_st_of None (tl_state_l S)\<close>
+    for S
+    by (cases S) (auto simp: tl_state_l_def tl_state_def convert_lits_l_def map_tl)
+  have twl_list_invs_tl_state_l: \<open>twl_list_invs S \<Longrightarrow> twl_list_invs (tl_state_l S)\<close> for S
+    by (cases S, cases \<open>get_trail_l S\<close>) (auto simp: tl_state_l_def twl_list_invs_def)
+  have clauses_to_update_l_tl_state: \<open>clauses_to_update_l (tl_state_l S) = clauses_to_update_l S\<close>
+    for S
+    by (cases S, cases \<open>get_trail_l S\<close>) (auto simp: tl_state_l_def)
+
   have H:
-    \<open>(skip_and_resolve_loop_l, skip_and_resolve_loop) \<in>
-    ?R \<rightarrow>
-    \<langle>{(T, T'). T' = twl_st_of None T \<and> twl_list_invs T \<and> clauses_to_update_l T = {#}}\<rangle> nres_rel\<close>
+    \<open>(skip_and_resolve_loop_l, skip_and_resolve_loop) \<in> ?R \<rightarrow>
+      \<langle>{(T::'v twl_st_l, T'). T' = twl_st_of None T \<and> twl_list_invs T \<and>
+        clauses_to_update_l T = {#}}\<rangle> nres_rel\<close>
     supply [[goals_limit=1]]
     unfolding skip_and_resolve_loop_l_def skip_and_resolve_loop_def
-    apply (refine_rcg get_conflict_l_get_conflict_state_spec H; remove_dummy_vars)
+    apply (refine_vcg get_conflict_l_get_conflict_state_spec H)
     subgoal by auto \<comment> \<open>conflict is not none\<close>
     subgoal by auto \<comment> \<open>loop invariant init: @{term skip_and_resolve_loop_inv}\<close>
     subgoal by auto \<comment> \<open>loop invariant init: @{term twl_list_invs}\<close>
@@ -1442,7 +1452,11 @@ proof -
     subgoal by (auto simp: is_decided_no_proped_iff lit_hd_get_trail_twl_st_of
       dest!: skip_and_resolve_loop_inv_trail_nempty)
     subgoal by simp
-    subgoal by (rule skip_and_resolve_l_refines) assumption+
+    subgoal by (auto simp: is_decided_no_proped_iff lit_hd_get_trail_twl_st_of
+      dest!: skip_and_resolve_loop_inv_trail_nempty)
+    subgoal by (auto simp: twl_list_invs_tl_state_l
+      dest!: skip_and_resolve_loop_inv_trail_nempty)
+    subgoal by (auto simp: clauses_to_update_l_tl_state)
     subgoal by auto
     subgoal by (rule skip_and_resolve_skip_refine)
         (auto simp: skip_and_resolve_loop_inv_def get_trail_twl_st_of_nil_iff)
@@ -2021,13 +2035,15 @@ definition cdcl_twl_o_prog_l :: \<open>'v twl_st_l \<Rightarrow> (bool \<times> 
       do {
         if get_conflict_l S = None
         then decide_l_or_skip S
-        else do {
+        else if count_decided (get_trail_l S) > 0
+        then do {
           T \<leftarrow> skip_and_resolve_loop_l S;
           ASSERT(get_conflict_l T \<noteq> None);
           if get_conflict_l T \<noteq> Some {#}
           then do {U \<leftarrow> backtrack_l T; RETURN (False, U)}
-          else do {RETURN (True, T)}
+          else RETURN (True, T)
         }
+        else RETURN (True, S)
       }
     }
   \<close>
@@ -2044,7 +2060,7 @@ lemma cdcl_twl_o_prog_l_spec:
        clauses_to_update_l S = {#} \<and> literals_to_update_l S = {#} \<and> no_step cdcl_twl_cp (twl_st_of None S) \<and>
        twl_struct_invs (twl_st_of None S) \<and> twl_stgy_invs (twl_st_of None S) \<and> twl_list_invs S} \<rightarrow>
     \<langle>{((brk, T), (brk', T')). T' = twl_st_of None T \<and> brk = brk' \<and> twl_list_invs T \<and> clauses_to_update_l T = {#} \<and>
-    (get_conflict_l T \<noteq> None \<longrightarrow> get_conflict_l T = Some {#})\<and>
+    (get_conflict_l T \<noteq> None \<longrightarrow> count_decided (get_trail_l T) = 0)\<and>
        twl_struct_invs (twl_st_of None T) \<and> twl_stgy_invs (twl_st_of None T) (* \<and>
        (\<not>brk \<longrightarrow> literals_to_update_l T \<noteq> {#}) *)}\<rangle> nres_rel\<close>
   (is \<open> _ \<in> ?R \<rightarrow> ?I\<close> is \<open> _ \<in> ?R \<rightarrow> \<langle>?J\<rangle>nres_rel\<close>)
@@ -2063,6 +2079,8 @@ proof -
     for M N U NE UE WS L and S' and D
     using that by (cases \<open>L\<close>) (auto intro!: rhs_step_bind_SPEC)
   have [simp]: \<open>literals_to_update (twl_st_of None T) = literals_to_update_l T\<close> for T
+    by (cases T) auto
+  have [simp]: \<open>count_decided (get_trail  (twl_st_of None T)) = count_decided (get_trail_l T)\<close> for T
     by (cases T) auto
   have twl_prog:
     \<open>(cdcl_twl_o_prog_l, cdcl_twl_o_prog) \<in> ?R \<rightarrow>
@@ -2104,11 +2122,15 @@ proof -
     subgoal by fast
     subgoal by fast
     subgoal
-      by (rule twl_st_lE) auto
+      by (simp del: split_paired_All)
     subgoal
       by (auto simp add: twl_list_invs_def)
     subgoal
       by fast
+    subgoal
+      by auto
+    subgoal
+      by auto
     subgoal
       by auto
     subgoal
@@ -2128,7 +2150,7 @@ proof -
       apply unify_Down_invs2+
       apply (simp only: nf set)
       apply ("match_\<Down>")
-      subgoal by force
+      subgoal by (cases S, clarsimp simp del: split_paired_All)
       subgoal by fast
       done
     done
@@ -2137,14 +2159,21 @@ qed
 
 subsection \<open>Full Strategy\<close>
 
+term cdcl_twl_stgy_prog_inv
+
+abbreviation cdcl_twl_stgy_prog_l_inv :: \<open>'v twl_st_l \<Rightarrow> bool \<times> 'v twl_st_l  \<Rightarrow> bool\<close> where
+  \<open>cdcl_twl_stgy_prog_l_inv S\<^sub>0 \<equiv> \<lambda>(brk, T). twl_struct_invs (twl_st_of None T) \<and>
+        twl_stgy_invs (twl_st_of None T) \<and>
+        (brk \<longrightarrow> final_twl_state (twl_st_of None T)) \<and>
+        cdcl_twl_stgy\<^sup>*\<^sup>* (twl_st_of None S\<^sub>0) (twl_st_of None T) \<and>
+        clauses_to_update_l T = {#} \<and>
+        (\<not>brk \<longrightarrow> get_conflict_l T = None)\<close>
+
 definition cdcl_twl_stgy_prog_l :: \<open>'v twl_st_l \<Rightarrow> 'v twl_st_l nres\<close> where
   \<open>cdcl_twl_stgy_prog_l S\<^sub>0 =
   do {
     do {
-      (brk, T) \<leftarrow> WHILE\<^sub>T\<^bsup>\<lambda>(brk, T). twl_struct_invs (twl_st_of None T) \<and> twl_stgy_invs (twl_st_of None T) \<and>
-        (brk \<longrightarrow> no_step cdcl_twl_stgy (twl_st_of None T)) \<and> cdcl_twl_stgy\<^sup>*\<^sup>* (twl_st_of None S\<^sub>0) (twl_st_of None T) \<and>
-        clauses_to_update_l T = {#} \<and>
-        (\<not>brk \<longrightarrow> get_conflict_l T = None)\<^esup>
+      (brk, T) \<leftarrow> WHILE\<^sub>T\<^bsup>cdcl_twl_stgy_prog_l_inv S\<^sub>0\<^esup>
         (\<lambda>(brk, _). \<not>brk)
         (\<lambda>(brk, S).
         do {
@@ -2214,7 +2243,8 @@ lemma cdcl_twl_stgy_prog_l_spec_final:
     \<open>clauses_to_update_l S = {#}\<close> and
     \<open>get_conflict_l S = None\<close> and \<open>twl_list_invs S\<close>
   shows
-    \<open>cdcl_twl_stgy_prog_l S \<le> SPEC(\<lambda>T. full cdcl_twl_stgy (twl_st_of None S) (twl_st_of None T))\<close>
+    \<open>cdcl_twl_stgy_prog_l S \<le> SPEC(\<lambda>T. cdcl_twl_stgy\<^sup>*\<^sup>* (twl_st_of None S) (twl_st_of None T) \<and>
+       final_twl_state (twl_st_of None T))\<close>
   apply (rule order_trans[OF cdcl_twl_stgy_prog_l_spec[THEN refine_pair_to_SPEC,
           of S \<open>twl_st_of None S\<close>]])
   using assms apply auto[2]
@@ -2222,6 +2252,7 @@ lemma cdcl_twl_stgy_prog_l_spec_final:
    apply (rule ref_two_step[OF _ cdcl_twl_stgy_prog_spec[of \<open>twl_st_of None S\<close>],
         of _ \<open>{(S, S'). S' = twl_st_of None S \<and> True}\<close>])
   using assms by (auto simp: full_def literals_to_update_l_literals_to_update
-      get_conflict_l_get_conflict pw_conc_inres pw_conc_nofail pw_ords_iff(1))
+      get_conflict_l_get_conflict pw_conc_inres pw_conc_nofail pw_ords_iff(1)
+    simp del: twl_st_of.simps)
 
 end
